#+LATEX_HEADER_EXTRA: \usepackage{indentfirst}
#+LATEX_HEADER_EXTRA: \usepackage{amsmath}
#+LATEX_HEADER_EXTRA: \usepackage{mathmode}

* Limits by the Definition

* Solution 1

  $\lim_{x \to 3} 2x - 4 = 3$

  Suppose $\epsilon > 0$. Let $\delta = \dfrac{\epsilon}{2} > 0$

  Suppose  $0 < |x-3| < \delta$

  $|2x - 4 - 2|$ = |2||x - 3|

  From $0 < |x-3| < \delta$, $|2||x - 3| < 2\delta$

  $|2||x - 3| < 2 \dfrac{\epsilon}{2}$

  $|2||x - 3| < \epsilon$

  Hence, $f(x) - L < \epsilon$

* Solution 2  

  $\lim_{t \to 1} 5 - 3t = 2$

  Suppose $\epsilon > 0$. Let $\delta = \dfrac{\epsilon}{3} > 0$  

  Suppose  $0 < |t-1| < \delta$

  $|5 - 3t - 2| = |3||1 - t|$

  From $0 < |t-1| < \delta$, $|3||t - 1| < 3\delta$

  $|3||t - 1| < \epsilon$

  Hence, $f(x) - L < \epsilon$

* Solution 3

  $\lim_{x \to -2}$ \dfrac{x^2 - 4}{x + 2} = -4$

  Suppose $\epsilon > 0$. Let $\delta = \epsilon > 0$

  Suppose  $0 < |x-(-2)| < \delta$

  $|\dfrac{x^2 - 4}{x + 2} + 4| = |x + 2| = |x - (-2)| < \delta$

  Hence, $f(x) - L < \epsilon$

* Solution 4

  $\lim_{x \to 2} \dfrac{x^2 - x - 2}{x - 2} = 3$
  
  Suppose $\epsilon > 0$. Let $\delta = \epsilon > 0$

  Suppose  $0 < |x-2| < \delta$

  Since $|x - 2| > 0$, $x \neq 2$ and hence the function is defined.

  $| \dfrac{x^2 - x - 2}{x - 2} - 3| = |x - 2|$

  We know that $|x - 2| < \delta$, So, $|x - 2| < \epsilon $

* Solution 5

  $\lim_{r \to 3} \dfrac{3r^2 - 8r - 3}{2r - 6} = 5$

  Suppose $\epsilon > 0$. Let $\delta = \dfrac{2}{3}\epsilon > 0$  

  Suppose  $0 < |r-3| < \delta$

  Since $0 < |r-3|$, $r \neq 3$ and hence the function is defined.

  $|\dfrac{3r^2 - 8r - 3}{2r - 6} - 5| = |\dfrac{3}{2}(r - 3)|$

  We know that $| r - 3 | < \delta$

  $|\dfrac{3}{2}(r - 3) | < \dfrac{3}{2}\delta < \epsilon$

* Solution 6

  $\lim_{x \to 2} \dfrac{x^2 + 2x - 8}{3x - 6} = 2$

  Suppose $\epsilon > 0$. Let $\delta = 2\epsilon > 0$  
  
  Suppose  $0 < |x-2| < \delta$

  Since $0 < |x-2|$, $x \neq 2$ and hence the function is defined.

  $|\dfrac{x^2 + 2x - 8}{3x - 6} - 2| = \dfrac{1}{2}(x - 2)$

  We know that $|x - 2| < \sigma$

  $\dfrac{1}{2}(x - 2) < 2.\dfrac{\epsilon}{2}$

  $\dfrac{1}{2}(x - 2) < \epsilon$

* Solution 7

  $\lim_{u \to -1} \dfrac{u^2 + 4u + 3}{u + 1} + u = 1$

  Suppose $\epsilon > 0$. Let $\delta = \dfrac{\epsilon}{2} > 0$  
  
  Suppose  $0 < |u-(-1)| < \delta$

  Since $|u-(-1)| > 0$, $u \neq -1$ and hence the function is defined.

  $\dfrac{u^2 + 4u + 3}{u + 1} + u - 1| = |2||u+1|$

  We know that $|u - (-1)| < \delta$

  $2 |u + 1| < 2\delta$

  $2 |u + 1| < \epsilon$

* Solution 8

  Suppose $\epsilon > 0$. Let $\delta = min(1, \dfrac{\epsilon}{2})$

  Notice that we have $\delta > 0, \delta \leq 1 and \delta \leq \dfrac{\epsilon}{2}$.

  Now suppose $0 < |x-2| < \delta$. Then,

  $|x - 2| < \delta \leq 1$. So, $0 < x - 1 < 2$.

  Thus, $|x^2 - 3x + 5 - 3| = |(x - 1)(x-2)| < 2|(x - 2)| < 2\delta < 2\dfrac{\epsilon}{2} = \epsilon$

* Solution 9

  Suppose $\epsilon > 0$. Let $\delta = min(\dfrac{1}{2}, \dfrac{\epsilon}{12})$

  Notice that we have $\delta > 0, \delta \leq \dfrac{1}{2} and \delta \leq \dfrac{\epsilon}{12}$.

  Now suppose $0 < |v-1| < \delta$. Then,

  $|v - 1| < \delta \leq \dfrac{1}{2}$. So, $1 < 2v < 3$.

  From $1 < 2v$, we infer $\dfrac{1}{3v - 1} < 2$.

  Thus, $|\dfrac{4}{3v - 1} - 2| = |\dfrac{6(v-1)}{1 - 3v}| = |\dfrac{6(v-1)}{3v - 1}| < 6(v-1)*2 <= 12\sigma <= 12\dfrac{\epsilon}{2} = \epsilon$

* Solution 10

  Suppose $\epsilon > 0$. Let $\delta = min(1, \epsilon)$

  Notice that we have $\delta > 0, \delta \leq 1 and \delta \leq \epsilon$.

  Now suppose $0 < |t-1| < \delta$. Then,

  $|t - 1| < \delta \leq 1$. So, $0 < t < 2$.

  From $0 < t$, we know that $\dfrac{1}{t + 1} < 1$

  Thus, $|\dfrac{2 - 2t}{t^2 - 1} + 1| = |\dfrac{t - 1)}{t + 1}| < |t-1| < \delta \leq \epsilon$

* Solution 11

  Suppose $\epsilon > 0$. Let $\delta = 1$

  Now suppose $0 < |x -3| < 1$. Solving it, we get $1 < \dfrac{x}{2} < 2$

  Since $\lfloor \dfrac{x}{2} \rfloor$ is always an integer from its
  range of $1 < \dfrac{x}{2} < 2$, we can determinte that $\lfloor
  \dfrac{x}{2} \rfloor$ will be $1$.

  So, $|\lfloor \dfrac{x}{2} \rfloor - 1| = 0 < \epsilon$

* Solution 12

  Suppose $\epsilon > 0$. Let $\delta = min(2, \dfrac{\epsilon}{28})$. 

  Notice that we have $\delta > 0, \delta \leq 2 and \delta \leq \dfrac{\epsilon}{28}$.

  Now suppose $0 < |x-2| < \delta$. Then,

  $|x - 2| < \delta \leq 2$. So, $x^2 < 16$ and $2x < 8$.

  From $x^2 < 16$ and $2x < 8$, $x^2 + 2x < 24$. So, $x^2 + 2x + 4< 28$

  Thus, $|x^3 - 8| = |(x-2)(x^2 + 4 + 2x)| < |(x - 2)|28 < ||(x-2).28| < 28.\delta <= 28\dfrac{\epsilon}{28} = \epsilon$

* Solution 13

  Suppose $\epsilon > 0$. Let $\delta = min(1, \dfrac{3\epsilon}{2})$.

  Notice that we have $\delta > 0, \delta \leq 1 and \delta \leq \dfrac{3\epsilon}{2}$.

  Now suppose $0 < |w-2| < \delta$. Then,

  $|w-2| < \delta \leq 1$. So, From $1 < w$, we can infer that $\dfrac{1}{\sqrt{2w + 5} + 3} < \dfrac{1}{\sqrt{7} + 3}$

  We know that $\dfrac{1}{\sqrt{7} + 3} < \dfrac{1}{3}$

  So by using transitive property,

  $\dfrac{1}{\sqrt{2w + 5} + 3} < \dfrac{1}{3}$

  $|\sqrt{2w + 5} - 3| = |\dfrac{2(w - 2)}{\sqrt{2w + 5} + 3}|$

  ( Note that the trick in the above reduction is to multiply by $\dfrac{{\sqrt{2w + 5} + 3}}{{\sqrt{2w + 5} + 3}}$)

  $|\dfrac{2(w - 2)}{\sqrt{2w + 5} + 3}| < \dfrac{2(w-2)}{3} < \dfrac{2\delta}{3} \leq \dfrac{2.3\delta}{3.2} = \epsilon$

* Solution 14

  Suppose $\epsilon > 0$. Let $\delta = min(2, \dfrac{\epsilon}{8})$.

  Notice that we have $\delta > 0, \delta \leq 2 and \delta \leq \dfrac{\epsilon}{8}$.

  Now suppose $0 < |t-3| < \delta$. Then,

  $|t^2 - 9| = |(t+3)(t-3)|$

  Since $|t-3| < \delta \leq 2$, we have $1 < t < 5$. Thus, $4 < t + 3 < 8$

  $(t+3)(t-3) = |t-3|(t+3) < 8|t-3| < 8\delta \leq \dfrac{8\epsilon}{8} = \epsilon$

* Solution 15

  Suppose $\epsilon > 0$. Let $\delta = min(1, \dfrac{\epsilon}{4})$.

  Notice that we have $\delta > 0, \delta \leq 1 and \delta \leq \dfrac{\epsilon}{4}$.

  Now suppose $0 < |x-1| < \delta$. Then,  $0 < x < 2$. So, $x + 2 < 4$.

  $|x^2 + x - 2| = |(x + 2)(x - 1)| < 4|x-1| < 4\delta \leq \dfrac{4\epsilon}{4} = \epsilon$

* Solution 16

  Suppose $\epsilon > 0$. Let $\delta = min(1, \dfrac{\epsilon}{9})$.

  Notice that we have $\delta > 0, \delta \leq 1 and \delta \leq \dfrac{\epsilon}{9}$.

  Now suppose $0 < |x-2| < \delta$. Then,  $1 < x < 3$. So, $3x < 9$.

  $|3x^2 - 6x - 0| = |3x(x-2)| < |x-2|9 < 9\delta <= \dfrac{9\epsilon}{9} = \epsilon$

* Solution 17

  Suppose $\epsilon > 0$. Let $\delta = min(3, \epsilon)$.  

  Notice that we have $\delta > 0, \delta \leq 3 and \delta \leq \epsilon$.

  Now suppose $0 < |x-(-1)| < \delta$. Then,  $\delta \leq 3$. So, $|x-(-1)| < 3$ and therefore $x-1<1$.

  $|\dfrac{x^3 + x^2 -3x - 3}{x+1} + 2| = |x^2 - 1| = |(x-1)(x+1)| < |x+1| < |x - (-1)| < \delta = \epsilon$

* Solution 18

  Suppose $\epsilon > 0$. Let $\delta = min(1, \dfrac{\epsilon}{2})$.

  Notice that we have $\delta > 0, \delta \leq 1 and \delta \leq \dfrac{\epsilon}{2}$.

  Now suppose $0 < |u-3| < \delta$. Then since,  $\delta \leq 1$. we have $2 < u <4$ and therefore $\dfrac{1}{u-1} < 1$.

  $|\dfrac{4}{u-1} - 2| = $\dfrac{2(u-3)}{u-1}| < |2(u-3)| < 2\delta < \dfrac{2\epsilon}{2} = \* 

* Solution 19

  Suppose $\epsilon > 0$. Let $\delta = min(4, \dfrac{\epsilon}{2})$.

  Notice that we have $\delta > 0, \delta \leq 4 and \delta \leq \dfrac{\epsilon}{2}$.

  Now suppose $0 < |t-5| < \delta$. Then since,  $\delta \leq 4$. we have $1 < t <9$ and therefore $\dfrac{1}{t} < 1$.

  $|\dfrac{3t - 10}{t} - 1| = |\dfrac{2(t-5)}{t}| < 2(t-5) < 2\delta \leq \dfrac{2\epsilon}{2} = \epsilon$

* Solution 20

  Suppose $\epsilon > 0$. Let $\delta = min(3, \sqrt{\dfrac{15\epsilon}{2}})$.

  Notice that we have $\delta > 0, \delta \leq 2 and \delta \leq \dfrac{15\epsilon}{2}$.
  
  Now suppose $0 < |z-1| < \delta$. Then since,  $\delta \leq 3$. we have $-3 < z-1 <3$ and therefore $9 < (z-1)^2, 1 < (z + 1)^2 and -7 < z - 5$

  $|\dfrac{z-1}{2z^2 + z - 3} - \dfrac{1}{5}| = |\dfrac{-2(z-1)^2}{5((z+1)^2 + (z-1)^2 + (z - 5))}|$

  We know that, $\dfrac{1}{(z-1)^2+(z+1)^2 + (z-5)} < \dfrac{1}{3}$

  $|\dfrac{-2(z-1)^2}{5((z+1)^2 + (z-1)^2 + (z - 5))}| < \dfrac{-2(z-1)^2}{5}\dfrac{1}{3} < \dfrac{2\delta^2}{16} \leq \epsilon$

* Solution 21

  Suppose $\epsilon > 0$. Let $\delta = min(1, \dfrac{\epsilon}{4})$.

  Notice that we have $\delta > 0, \delta \leq 1 and \delta \leq \dfrac{\epsilon}{4}$.

  Now suppose $0 < |y-1| < \delta$. Then since,  $\delta \leq 1$. we have $0 < y <2$ and therefore $y^2 < 4$

  $|y^3 - y^2 + 7 = 7| = |y^2(y-1)| < 4|y-1| < 4\delta \leq 4\dfrac{\epsilon}{4} = \epsilon$

* Solution 22

  Suppose $\epsilon > 0$. Let $\delta = min(1, \sqrt{\dfrac{\epsilon}{2}})$.

  Notice that we have $\delta > 0, \delta \leq 1 and \delta \leq \sqrt{\dfrac{\epsilon}{2}}$.

  Now suppose $0 < |y-0| < \delta$. Then since,  $\delta \leq 1$. we have $-1 < y <1$ and therefore $1-y < 2$

  $|y^3 - y^2 + 7 - 7| = |y^2(1-y)| < 2y^2 < 2\delta^2 \leq \epsilon$

* Solution 23

  Suppose $\epsilon > 0$. Let $\delta = min(1, 2(3 + \sqrt[2]{3})\epsilon)$.  

  Notice that we have $\delta > 0, \delta \leq 1$ and $\delta \leq 2(3 + \sqrt[2]{3})\epsilon$.

  Suppose $0 < |x-4| < \epsilon$. Then since, $\delta \leq 1$, we have $3 < x < 5$ and therefore $\dfrac{1}{x + 2\sqrt{x} < \dfrac{1}{3 + 2\sqrt{3}}}$

  $|\dfrac{1}{\sqrt{x}} - \dfrac{1}{2}| = \dfrac{-1(4-x)}{2(x + 2\sqrt{x})} < \dfrac{|-1(4-x)|}{2(3+2\sqrt{3})} < \dfrac{|4-x|}{2(x+2\sqrt{3})} < \dfrac{\epsilon}{2(3 + 2\sqrt{3})} \leq \epsilon$

* Solution 24

  Suppose $\epsilon > 0$. Let $\delta = min(1, \sqrt{\epsilon})$.

  Notice that we have $\delta > 0, \delta \leq 1$ and $\delta \leq \sqrt{\epsilon}$.

  Suppose $0 < |x-0| < \epsilon$. Then since, $\delta \leq 1$, we have $-1 < x < 1$ and therefore $\dfrac{1}{\sqrt{x^2 + 1}-1} < \dfrac{1}{\sqrt{2}-1} < 1$

  $|\sqrt{x^2 + 1} - 1| = |\dfrac{x^2}{\sqrt{x^2 + 1} + 1}| < |x^2| < \delta^2 \leq \epsilon$
