* Derivative Rules

** Theorem 3.3.1

Constant functions and the identity functions are differentiable at
all numbers, and their derivatives are given by the following
formulas:

- Suppose $f$ is a constant function; that is, there is some number
  $c$ such that $f(x)=c$. Then $f'(x)=0$. In other words,
  $\dfrac{d}{dx}(c) = 0$.
- Suppose $f$ is the identity function; that is, $f(x)=x$. Then
  $f'(x)=1$. In other words, $\dfrac{d}{dx}(x) = 1$.

** Theorem 3.3.2

Suppose that $f$ and $g$ are functions and $c$ is a number.

- If $f$ and $g$ are differentiable at a number $x$, then so is $f +
  g$, and

  $(f+g)'(x) = f'(x) + g'(x)$

  In other words,

  $\dfrac{d}{dx}(f(x)+g(x)) = \dfrac{d}{dx}(f(x)) + \dfrac{d}{dx}(g(x))$

- If $f$ is differentiable at $x$, then so is $cf$, and

  $(cf)'(x) = c(f'(x))$

  In other words,

  $\dfrac{d}{dx}(cf(x)) = c.\dfrac{d}{dx}(f(x))$

- If $f$ and $g$ are differentiable at a number $x$, then so is $f -
  g$, and

  $(f-g)'(x) = f'(x)-g'(x)$

  In other words,

  $\dfrac{d}{dx}(f(x)-g(x)) = \dfrac{d}{dx}(f(x)) - \dfrac{d}{dx}(g(x))$

** Theorem 3.3.3 (Product Rule)

If $f$ and $g$ are differentiable at $x$, then so is $fg$, and

$(fg)'(x) = f(x)g'(x) + g(x)f'(x)$

In other words,

$\dfrac{d}{dx}(f(x)g(x)) = f(x)\dfrac{d}{dx}(g(x)) + g(x)\dfrac{d}{dx}(f(x))$

** Theorem 3.3.4 (Power Rule)

Suppose $n$ is a positive integer, and $f(x) = x^n$. Then $f$ is
differentiable at all numbers, and $f'(x) = nx^{n-1}$. In other words,
$\dfrac{d}{dx} (x^n) = nx^{n-1}$.

** Theorem 3.3.5 (Quotient Rule)

If $f$ and $g$ are differentiable at $x$ and $g(x) \neq 0$, then $f/g$
is differentiable at $x$, and

$(f/g)'(x) = \dfrac{g(x)f'(x) - f(x)g'(x)}{(g(x))^2}$

In other words,

$\dfrac{d}{dx}(\dfrac{f(x)}{g(x)}) = \dfrac{g(x)\dfrac{d}{dx}(f(x)) - f(x)\dfrac{d}{dx}(g(x))}{(g(x))^2}$
  
** Theorem 3.3.6

   Suppose $n$ is a negative integer, and for all $x \neq 0, f(x) =
   x^n$. Then $f$ is differentiable at all $x \neq 0$, and $f'(x) =
   nx^{n-1}$. In other words, $\dfrac{d}{dx}x^n = nx^{n-1}$.

** Theorem 3.3.7

   Suppose $n$ is an integer, $n \geq 2$, and $f(x) =
   x^{\dfrac{1}{n}}$. Then $f'(x) = \dfrac{1}{n}x^{\dfrac{1}{n} -
   1}$. If $n$ is even then the domain of $f'$ is $(0, \infty)$, and
   if $n$ is odd then it is $(-\infty,0) \cup (0, \infty)$.

   [[http://www.mesacc.edu/~scotz47781/mat120/notes/exponents/rational/rational_exponents.html][Ref 1: Definition of Radicals]]   
   
   [[http://www.mesacc.edu/~scotz47781/mat120/notes/radicals/domain/any_index/any_radical.html][Ref 2: Domain of Radical Functions]]


** Derivatives of trignometric functions

   $\dfrac{d}{dx}(\sin x) = \cos x$

   $\dfrac{d}{dx}(\cos x) = -\sin x$

   $\dfrac{d}{dx}(\tan x) = \sec^2 x$

   $\dfrac{d}{dx}(\cot x) = -\csc^2 x$

   $\dfrac{d}{dx}(\sec x) = \sec x \tan x$

   $\dfrac{d}{dx}(\csc x) = -\csc x \cot x$   
   

