* Implicit Differentiation

** Solution 1

   $f_b(x) = -\sqrt{1-x^2}$

   $f'_b(x) = \dfrac{-1}{x}(1-x^2)^{-1/2}(-2x)$

   $= \dfrac{-1}{2\sqrt{1-x^2}} * (-2x)$

   $= \dfrac{x}{\sqrt{1-x^2}}$

   $f'_b(3/5) = \dfrac{3/5}{\sqrt{1-(3/5)^2}}$

   $= \dfrac{3/5}{\sqrt{16/25}}$

   $= \dfrac{3/5}{4/5}$

   $= \dfrac{3}{4}$

** Solution 2

   $x^3 + y^3 = 1$

   Using implicit differentiation,

   $2x^2 + 3y^2\dfrac{dy}{dx} = 0$

   $3y^2\dfrac{dy}{dx} = -2x^2$

   $\dfrac{dy}{dx} = \dfrac{-2x^2}{3y^2}$

** Solution 3

   $x^{1/3} + y^{1/3} = 1$

   Using implicit differentiation,

   $\dfrac{1}{3}x^{1/3 - 1} + \dfrac{1}{3}y^{1/3-1}\dfrac{dy}{dx} = 0$

   $dfrac{1}{3}x^{-2/3} + \dfrac{1}{3}y^{-2/3}\dfrac{dy}{dx} = 0$

   $x^{-2/3} + y^{-2/3}\dfrac{dy}{dx} = 0$

   $y^{-2/3}\dfrac{dy}{dx} = -x^{-2/3}$

   $\dfrac{dy}{dx} = \dfrac{-x^{-2/3}}{y^{-2/3}}$

   $= \dfrac{-y^{2/3}}{x^{2/3}}$

** Solution 4

   $x^3y-y^3x = 3$

   Using implicit differentiation,

   $x^3\dfrac{dy}{dx} + y3x^2 - (y^3 + x3y^2\dfrac{dy}{dx}) = 0$

   $x^3\dfrac{dy}{dx} + 3x^2y - y^3 - 3xy^2\dfrac{dy}{dx} = 0$

   $x^3 \dfrac{dy}{dx} - 3xy^2\dfrac{dy}{dx} = y^3 - 3x^2y$

   $\dfrac{dy}{dx}(x^3 - 3xy^2) = y^3 - 3x^2y$

   $\dfrac{dy}{dx} = \dfrac{y^3-3x^2y}{x^3-3xy^2}$

** Solution 5

   $xy^2 + \sqrt{x+y} = 5$

   Using implicit differentiation,

   $y^2 + x.2y\dfrac{dy}{dx} + (x+y)^{-1/2}\dfrac{1}{2}(1 + \dfrac{dy}{dx}) = 0$

   $y^2 + 2xy\dfrac{dy}{dx} + \dfrac{1}{2\sqrt{x+y}}(1 + \dfrac{dy}{dx}) = 0$

   $y^2 + 2xy\dfrac{dy}{dx} + \dfrac{1}{2\sqrt{x+y}} + \dfrac{1}{2\sqrt{x+y}}\dfrac{dy}{dx} = 0$

   $y^2 + \dfrac{1}{2\sqrt{x+y}} + \dfrac{dy}{dx}(2xy + \dfrac{1}{2\sqrt{x+y}}) = 0$

   $\dfrac{dy}{dx} = \dfrac{-y^2 - \dfrac{1}{2\sqrt{x+y}}}{2xy + \dfrac{1}{2\sqrt{x+y}}}$

   $= \dfrac{-2y^2\sqrt{x+y} - 1}{2xy\sqrt{x+y} + 1}$

** Solution 6

   $x = \sin xy$

   Using implicit differentiation,

   $1 = \cos (xy) \dfrac{d}{dx} (xy)$

   $1 = \cos(xy)(x\dfrac{dy}{dx} + y)$

   $1 = x\cos(xy)\dfrac{dy}{dx} + y\cos(xy)$

   $x \cos(xy) \dfrac{dy}{dx} = 1 - y\cos(xy)$

   $\dfrac{dy}{dx} = \dfrac{1-y\cos(xy)}{x\cos(xy)}$

** Solution 7

   $y = \sin(xy)$

   Using implicit differentiation,

   $\dfrac{dy}{dx} = x\cos (xy)\dfrac{dy}{dx} + y\cos (xy)$

   $\dfrac{dy}{dx}(1-x\cos(xy)) = y \cos (xy)$

   $\dfrac{dy}{dx} = \dfrac{y\cos (xy)}{1 - x\cos(xy)}$

** Solution 8

   $y = cos (x/y)$

   Using implicit differentiation,

   $\dfrac{dy}{dx} = -\sin(x/y)\dfrac{d}{dx}(x/y)$

   $\dfrac{dy}{dx} = -\sin(x/y)\dfrac{y.1-x\dfrac{dy}{dx}}{y^2}$

   $\dfrac{dy}{dx} = -\sin(x/y)(\dfrac{1}{y} - \dfrac{x}{y^2}\dfrac{dy}{dx})$

   $\dfrac{dy}{dx} = \dfrac{-1}{y}\sin(x/y) + \dfrac{x}{y^2}\dfrac{dy}{dx}$

   $\dfrac{dy}{dx}(1 - \dfrac{x}{y^2}) = \dfrac{-1}{y}\sin(x/y)$

   $\dfrac{dy}{dx}(\dfrac{y^2-x}{y^2}) = \dfrac{-1}{y}\sin(\dfrac{x}{y})$

   $\dfrac{dy}{dx}(y^2 - x) = -y\sin(x/y)$

   $\dfrac{dy}{dx} = \dfrac{-y\sin (x/y)}{y^2 - x} = \dfrac{y\sin(x/y)}{x-y^2}$

** Solution 9

   $xy^2 = \sin(3x-y)$

   Using implicit differentiation,

   $\dfrac{d}{dx} (xy^2) = \cos(3x-y)(3 - \dfrac{dy}{dx})$

   $x.2y\dfrac{dy}{dx} + y^2 = \cos(3x-y)(3-\dfrac{dy}{dx})$

   $2xy\dfrac{dy}{dx} + y^2 = 3\cos(3x-y)-\cos(3x-y)\dfrac{dy}{dx}$

   $\dfrac{dy}{dx}(2xy+\cos(3x-y)) = 3\cos(3x-y)-y^2$

   $\dfrac{dy}{dx} = \dfrac{3\cos(3x-y)-y^2}{\cos(3x-y)+2xy}$

** Solution 10

   $y\tan(x-y) = x$

   Using implicit differentiation,

   $\dfrac{d}{dx}(y\tan(x-y)) = 1$

   $y\dfrac{d}{dx}(\tan(x-y)) + \tan(x-y)\dfrac{dy}{dx} = 1$

   $y\sec^2(x-y)(1-\dfrac{dy}{dx}) + \tan(x-y)\dfrac{dy}{dx} = 1$

   $y\sec^2(x-y)-y\sec^2(x-y)\dfrac{dy}{dx}+\tan(x-y)\dfrac{dy}{dx} = 1$

   $y\sec^2(x-y)+\dfrac{dy}{dx}(\tan(x-y)-y\sec^2(x-y)) = 1$

   $\dfrac{dy}{dx}(\tan(x-y)-y\sec^2(x-y)) = 1-\sec^2(x-y)$

   $\dfrac{dy}{dx}=\dfrac{1-\sec^2(x-y)}{\tan(x-y)-y\sec^2(x-y)}$

** Solution 11

   $y\sqrt{xy+3} = 2x$

   Using implicit differentiation,

   $\dfrac{d}{dx}(y\sqrt{xy+3}) = 2$

   $y\dfrac{d}{dx}(xy+3)^{1/2} + \sqrt{xy+3}\dfrac{dy}{dx} = 2$

   $\dfrac{y}{2(xy+3)^{1/2}} \dfrac{d}{dx}(xy+3) + \sqrt{xy+3}\dfrac{dy}{dx} = 2$

   $\dfrac{y}{2\sqrt{xy+3}}(x\dfrac{dy}{dx} + y) + \sqrt{xy+3}\dfrac{dy}{dx} = 2$

   $\dfrac{xy}{2\sqrt{xy+3}}\dfrac{dy}{dx} + \dfrac{y^2}{2\sqrt{xy+3}} + \sqrt{xy+3}\dfrac{dy}{dx} = 2$

   $\dfrac{dy}{dx}(\dfrac{xy}{2\sqrt{xy+3} + \sqrt{xy+3}}) = 2 - \dfrac{y^2}{2\sqrt{xy+3}}$

   $\dfrac{dy}{dx}(\dfrac{xy+2(xy+3)}{2\sqrt{xy+3}}) = \dfrac{4\sqrt{xy+3}-y^2}{2\sqrt{xy+3}}$

   $\dfrac{dy}{dx}(xy+2(xy+3)) = 4\sqrt{xy+3}-y^2$

   $\dfrac{dy}{dx} = \dfrac{4\sqrt{xy+3}-y^2}{3xy + y}$

   $= \dfrac{4.(2x/y) - y^2}{3xy+6}$

   $= \dfrac{8x-y^3}{3xy^2 + 6y}$

** Solution 12

   $y = x^2 + \sin y$

   Using implicit differentiation,

   $\dfrac{dy}{dx} = 2x + \cos y (\dfrac{dy}{dx})$

   $\dfrac{dy}{dx}(1-\cos y) = 2x$

   $\dfrac{dy}{dx} = \dfrac{2x}{1-\cos y}$

   $\dfrac{d^2y}{dx^2} = \dfrac{(1-\cosy)2 - 2x(0+\siny \dfrac{dy}{dx})}{(1-\cos y)^2}$

   $= \dfrac{2(1-\cos y)-2x(\sin y.\dfrac{dy}{dx})}{(1-\cos y)^2}$

   $= \dfrac{2(1-\cos y)-2x(\dfrac{\sin y 2x}{1-\cos y})}{(1-\cos y)^2}$

   $= \dfrac{2(1-\cos y)^2-2x(\sin y (2x))}{(1-\cos y)^3}$

   $= \dfrac{2(1-\cos y)^2 - 4x^2 \sin y}{(1-\cos y)^3}$

** Solution 13

   $y^2 = x - y$

   Using implicit differentiation,

   $2y \dfrac{dy}{dx} = 1 - \dfrac{dy}{dx}$

   $\dfrac{dy}{dx}(2y + 1) = 1$

   $\dfrac{dy}{dx} = \dfrac{1}{2y + 1}$

   $\dfrac{d^2y}{dx^2} = \dfrac{(2y+1).0 - 1(2\dfrac{dy}{dx})}{(2y+1)^2}$

   $= \dfrac{0 - 2\dfrac{dy}{dx}}{(2y+1)^2}$

   $= \dfrac{-2/(2y+1)}{(2y+1)^2}$

   $= \dfrac{-2}{(2y+1)^3}$

** Solution 14

   $y = \sqrt{xy + 1}$

   $\dfrac{dy}{dx} = \dfrac{1}{2}(xy + 1)^{-1/2}\dfrac{d}{dx}(xy + 1)$

   $\dfrac{dy}{dx} = \dfrac{1}{2\sqrt{xy + 1}}(x\dfrac{dy}{dx} + y)$

   $\dfrac{dy}{dx} = \dfrac{x}{2\sqrt{xy + 1}}\dfrac{dy}{dx} + \dfrac{y}{2\sqrt{xy + 1}}$

   $\dfrac{dy}{dx}(1 - \dfrac{x}{2\sqrt{xy + 1}}) = \dfrac{y}{2\sqrt{xy + 1}}$

   $\dfrac{dy}{dx}(\dfrac{2\sqrt{xy + 1}-x}{2\sqrt{xy + 1}}) = \dfrac{y}{2\sqrt{xy + 1}}$

   $\dfrac{dy}{dx} = \dfrac{y}{2\sqrt{xy + 1} - x}$

   $\dfrac{d^2y}{dx^2} = \dfrac{(2\sqrt{xy + 1}-x)\dfrac{dy}{dx} - y\dfrac{d}{dx}(2\sqrt{(xy + 1) - x})}{(2\sqrt{xy + 1} - x)^2}$

   $2\sqrt{xy + 1}-x)\dfrac{dy}{dx} = (2\sqrt{xy + 1} - x)\dfrac{y}{2\sqrt{xy + 1}-x} = y$

   $y\dfrac{d}{dx}(2\sqrt{(xy + 1) - x})$

   $= \dfrac{2y}{2\sqrt{xy+1}} \dfrac{d}{dx} (xy + 1) - y$

   $= \dfrac{y}{\sqrt{xy + 1}} \dfrac{d}{dx} (xy + 1) - y$

   $= \dfrac{y}{\sqrt{xy + 1}}(x \dfrac{dy}{dx} + y) - y$

   $= \dfrac{xy}{\sqrt{xy + 1}} \dfrac{dy}{dx} + \dfrac{y^2}{\sqrt{xy + 1}} - y$

   $= \dfrac{xy}{\sqrt{xy + 1}}\dfrac{y}{(2\sqrt{xy + 1}) - x} + \dfrac{y^2}{\sqrt{xy + 1}} - y$

   $= \dfrac{xy^2}{\sqrt{xy + 1}(2\sqrt{xy + 1} - x)} + \dfrac{y^2}{\sqrt{xy + 1}} - y$

   Removing the $y$, we get

   $= \dfrac{xy^2}{\sqrt{xy + 1}(2\sqrt{xy + 1} - x)} + \dfrac{y^2}{\sqrt{xy + 1}}$

   $= \dfrac{xy^2 + y^2(2\sqrt{xy + 1}-x)}{\sqrt{xy + 1}(2\sqrt{xy + 1} - x)}$

   $\dfrac{d^2y}{dx^2} = \dfrac{xy^2 + y^2(2\sqrt{xy + 1}-x)}{\sqrt{xy + 1}(2\sqrt{xy + 1} - x)}$

** Solution 15

   $x^{2/3} + y^{2/3} = 1$

   $\dfrac{2}{3}x^{-1/3} + \dfrac{2}{3}y^{-1/3}\dfrac{dy}{dx} = 0$

   $\dfrac{2}{3}y^{-1/3}\dfrac{dy}{dx} = \dfrac{-2}{3}x^{-1/3}$

   $y^{-1/3}\dfrac{dy}{dx} = -x^{-1/3}$

   $\dfrac{dy}{dx} = \dfrac{-x^{-1/3}}{y^{-1/3}} = \dfrac{-y^{1/3}}{x^{1/3}}$

   $\dfrac{d^2y}{dx^2} = \dfrac{-x^{1/3}\dfrac{d}{dx}(y^{1/3}) + y^{1/3}\dfrac{1}{3}x^{-2/3}}{x^{2/3}}$

   $= \dfrac{\dfrac{-x^{1/3}}{3y^{2/3}}\dfrac{dy}{dx} + \dfrac{y^{1/3}}{x^{2/3}}\dfrac{1}{3}}{x^{2/3}}$

   $= \dfrac{\dfrac{y^{1/3}}{3y^{2/3}} + \dfrac{1y^{1/3}}{3x^{2/3}}}{x^{2/3}}$

   $= \dfrac{y^{1/3}}{3y^{2/3}x^{2/3}} + \dfrac{y^{1/3}}{3x^{4/3}}$

   $= \dfrac{y^{1/3}}{3x^{4/3}} + \dfrac{1}{3x^{2/3}y^{1/3}}$

   $= \dfrac{y^{2/3}}{3x^{4/3}y^{1/3}} + \dfrac{x^{2/3}}{3x^{4/3}y^{1/3}}$

   $= \dfrac{y^{2/3} + x^{2/3}}{3x^{4/3}y^{1/3}}$

   $= \dfrac{1}{3x^{4/3}y^{1/3}}$

** Solution 16

   $xy^2 = x + y$

   Using implicit differentiation,

   $x2y \dfrac{dy}{dx} + y^2 = 1 + \dfrac{dy}{dx}$

   $\dfrac{dy}{dx} (2xy - 1) = 1 - y^2$

   $\dfrac{dy}{dx} = \dfrac{1-y^2}{2xy - 1}$

   $\dfrac{d^2y}{dx^2} = \dfrac{(2xy - 1)\dfrac{d}{dx}(1-y^2)-(1-y^2)\dfrac{d}{dx}(2xy - 1)}{(2xy-1)^2}$

   $= \dfrac{(2xy-1)(-2y\dfrac{dy}{dx}) - (1-y^2)(2x\dfrac{dy}{dx} + 2y)}{(2xy-1)^2}$

   $(2xy - 1)(-2y\dfrac{dy}{dx}) = (2xy-1)(-2y)\dfrac{(1-y^2)}{(2xy-1)}$

   $= 2y(y^2 - 1)$

   $(1-y^2)(2x\dfrac{dy}{dx} + 2y) = 2x\dfrac{dy}{dx} + 2y - 2xy^2\dfrac{dy}{dx} - 2y^3$

   $= 2y - 2y^3 + \dfrac{dy}{dx}(2x - 2xy^2)$

   $= 2y- 2y^3 + \dfrac{dy}{dx}2x(1-y^2)$

   $= 2y - 2y^3 + \dfrac{2x(1-y^2)^2}{2xy - 1}$

   $= 2y(y^2 -1)-(2y - 2y^3 + \dfrac{2x(1-y^2)^2}{(2xy-1)})$

   $= 2y^3 - 2y - 2y + 2y^3 + \dfrac{2x(1-y^2)^2}{2xy - 1}$

   $= 4y^3 - 4y + \dfrac{2x(1-y^2)^2}{2xy - 1}$

   $= 4y(y^2 - 1) + \dfrac{2x(1-y^2)^2}{2xy - 1}$

   $\dfrac{d^2y}{dx^2} = \dfrac{4y(y^2-1)}{(2xy-1)^2} + \dfrac{2x(1-y)^2}{(2xy-1)^3}$

** Solution 17

   $y = f(x)$

   $\dfrac{dy}{dx} = \dfrac{y^2+3}{2x}$

   $\dfrac{d^2y}{dx^2} = \dfrac{2x\dfrac{d}{dx}(y^2 + 3) - (y^2 + 3).2}{(2x)^2}$

   $= \dfrac{2x(2y\dfrac{dy}{dx}) - 2(y^2 + 3)}{4x^2}$

   $= \dfrac{y}{x}\dfrac{dy}{dx} - \dfrac{2(y^2+3)}{4x^2}$

   $= \dfrac{y(y^2+3)}{x(2x)} - \dfrac{2(y^2+3)}{4x^2}$

   $= \dfrac{y(y^2+3)}{x(2x)} - \dfrac{2(y^2 + 3)}{4x^2}$

   $= \dfrac{y(y^2 + 3)}{2x^2} - \dfrac{2(y^2 + 3)}{4x^2}$

   $= \dfrac{2y(y^2 + 3)}{4x^2} - \dfrac{2(y^2 + 3)}{4x^2}$

   $= \dfrac{2y(y^2 + 3) - 2(y^2 + 3)}{4x^2}$

   $= \dfrac{2(y^2 + 3)(y-1)}{4x^2}$

   $= \dfrac{(y^2 + 3)(y-1)}{2x^2}$

** Solution 18

   $\sin (xy) = \cos (x + y)$

   Find equation of line tangent at $(\pi/2, 0)$

   Using implicit differentiation,

   $\cos (xy) \dfrac{d}{dx}(xy) = -\sin(x+y)\dfrac{d}{dx}(x + y)$

   $\cos (xy)(x \dfrac{dy}{dx} + y) = -\sin(x+y)(1 + \dfrac{dy}{dx})$

   $x\dfrac{dy}{dx}\cos (xy) + y\cos (xy) = -\sin(x+y) - \dfrac{dy}{dx}\sin(x+y)$

   $x\dfrac{dy}{dx}\cos (xy) + \dfrac{dy}{dx}\sin (x+y) = -\sin(x+y) -y\cos (xy)$

   $\dfrac{dy}{dx}(x\cos (xy) + \sin(x+y)) = -\sin(x+y)-y\cos(xy)$

   $\dfrac{dy}{dx} = \dfrac{-\sin(x+y)-y\cos(xy)}{\sin(x+y)+x\cos (xy)}$


   $\dfrac{dy}{dx}\Bigr|_(x,y)=(\pi/2,0) = \dfrac{-\sin(\pi/2)-0}{\sin(\pi/2)+(\pi/2)\cos 0}$

   $= \dfrac{-1}{1 + \pi/2}$

   $= \dfrac{-2}{\pi + 2}$

   Equation of line

   $m = \dfrac{y-y_1}{x-x_1}$

   $\dfrac{-2}{\pi + 2} = \dfrac{y - 0}{x - \pi/2}$

   $\dfrac{-2}{\pi + 2} = \dfrac{2y}{2x - \pi}$

   $\dfrac{-1}{\pi + 2} = \dfrac{y}{2x - \pi}$

   $\pi - 2x = y(\pi + 2)$

   $y(\pi + 2) + 2x = \pi$

** Solution 19

   Equation of curve: $\cos (x^2y) + 3y = c$

   Curve passes through $(2, \pi/8)$

*** Solution a

    $P = (2, \pi/8)$

    $x^2y= 2^2 \dfrac{\pi}{8} = \dfrac{\pi}{2}$

    $c = \cos (\pi / 2) + 3\pi/8 = 3\pi/8$

*** Solution b

    $P = (2, \pi/8)$

    $\cos (x^2y) + 3y = \dfrac{3\pi}{8}$

    Using implicit differentiation,

    $-\sin(x^2y)\dfrac{d}{dx}(x^2y) + 3\dfrac{dy}{dx} = 0$

    $-\sin(x^2y)(x^2\dfrac{dy}{dx} + y2x) + 3\dfrac{dy}{dx} = 0$

    $-x^2\sin(x^2y)\dfrac{dy}{dx} - 2xy \sin(x^2y) + 3\dfrac{dy}{dx} = 0$

    $\dfrac{dy}{dx}(3-x^2(\sin (x^2y))) = 2xy\sin(x^2y)$

    $\dfrac{dy}{dx} = \dfrac{2xy\sin(x^2y)}{3-x^2\sin(x^2y)}$

    $\dfrac{dy}{dx}\Bigr|_(x,y)=(2,\pi/8) = \dfrac{\pi/2 \sin(\pi/2)}{3-4\sin(\pi/2)}$

    $= \dfrac{\pi/2}{3-4}$

    $= \dfrac{\pi/2}{-1}$

    $= \dfrac{-\pi}{2}$

    $m = \dfrac{y-\pi/8}{x-2}$

    $\dfrac{-\pi}{2} = \dfrac{8y-\pi}{8(x-2)}$

    $-4\pi = \dfrac{8y-\pi}{x-2}$

    $-4\pi x + 8\pi = 8y - \pi$

    $9\pi - 4\pi x = 8y$

    $y = \dfrac{-\pi x}{2} + \dfrac{9\pi}{8}$

** Solution 20

   $y = \dfrac{2\sin x + \cos y}{3}$

   $a_{n+1} = \dfrac{2\sin(\pi/6) + \cos a_n}{3}$

   $= \dfrac{1 + \cos a_n}{3}$

*** Solution a

    $|a_n - f(\pi/6)| \leq 1/3^n$

    We will prove using mathematical inducation.

    Base case: $n = 1$

    $a_1 = \dfrac{1}{3}$

    $f(\pi/6) = \dfrac{2\sin(\pi/6) + \cos y}{3} = \dfrac{1 + \cos y}{3}$

    Range of $f(\pi/6) = [0, 2/3]$

    So, $|a_1 - f(\pi/6)| \leq 1/3$

    Induction step: Let $n$ be a positive integer and $|a_n -
    f(\pi/6)| \leq 1/3^n$.

    Suppose $|a_{n+1} - f(\pi/6)|$.

    $= |\dfrac{1 + \cos a_n}{3} - \dfrac{1 + \cos (f(\pi/6))}{3}|$

    $= |\dfrac{\cos a_n - \cos (f(\pi/6))}{3}|$

    $= \dfrac{|\cos a_n - \cos (f(\pi/6))|}{3}$

    $= \dfrac{|a_n - f(\pi/6)|}{3}$ (From Lemma 9)

    $ \leq \dfrac{1/3^n}{3} \leq \dfrac{1}{3^{n+1}}$

    That concludes the mathematical induction proof.

*** Solution b

    $\lim_{n \to \infty} a_n = f(\pi/6)$

    From (a), we know that $\forall n $|a_n - f(\pi/6)| \leq 1/3^n$$

    We know that $n$ is a positive integer.

    Suppose $\epsilon = \dfrac{1}{3^n - 1}$

    Suppose $\exists N$ such that $n > N$

    Since $$|a_n - f(\pi/6)| \leq 1/3^n$ < \dfrac{1}{3^{n-1}}$

    So, $\lim_{n \to \infty} a_n = f(\pi/6)$

*** Solution c

    $\dfrac{1}{3^n} = 0.005$

    $3^n = \dfrac{1}{0.005}$

    $3^n = \dfrac{1000}{5}$

    $3^n = 200$

    $n \approx 4.8$

    So at $n=5$, we know that $a_n$ differes from $f(\pi/6)$ by at
    most $0.005$

    $a_1 = 1/3$

    $a_2 = \dfrac{1 + \cos (1/3)}{3} = 0.6483$

    $a_3 = \dfrac{1 + \cos(0.6483)}{3} = 0.59903$

    $a_4 = \dfrac{1 + \cos (0.59903)}{3} = 0.60862$

    $a_5 = \dfrac{1 + \cos (0.60962)}{3} = 0.60681$

    $a_5 = 0.60681$

