* The Chain Rule

** Solution 1

   $f(x) = (5x-8)^{12}$

   $f'(x) = 12(5x-8)^{11} \dfrac{d}{dx} (5x-8)$

   $= 12(5x - 8)^{11}.5$

   $= 60(5x-8)^{11}$

** Solution 2

   $g(x) = \sin (x^2 + 7x-9)$

   $g'(x) = \cos (x^2 + 7x - 9) (2x+7)$

   $= (2x+7)\cos (x^2 + 7x - 9)$

** Solution 3

   $h(x) = \sqrt{x^2 + 4}$

   $h'(x) = \dfrac{1}{2}(x^2 + 4)^{-1/2}(2s)$

   $= \dfrac{x}{\sqrt{x^2 + 4}}$

** Solution 4

   $f(x) = x^3 \tan (x^2 + 3x)$

   Using the product rule,

   $f'(x) = x^3 \dfrac{d}{dx}(\tan (x^2 + 3x)) + \tan(x^2 + 3x)(3x^2)$

   $= x^3 \sec^2 (x^2 + 3x)(2x+3) + 3x^2 \tan(x^2 + 3x)$

   $= (2x^4 + 3x^3)\sec^2 (x^2 + 3x) + 3x^2 + \tan(x^2 + 3x)$

** Solution 5

   $h(x) = \dfrac{2}{\sqrt[3]{3x+4}}$

   $h(x) = 2(3x+4)^{-1/3}$

   $h'(x) = 2 * \dfrac{-1}{3} * (3x + 4)^{-1/3 - 1}.*h3$

   $= -2(3x+4)^{-4/3}$

   $= \dfrac{-2}{(3x+4)^{4/3}}$

   $= \dfrac{-2}{\sqrt[3]{(3x+4)^4}}$

** Solution 6

   $g(x) = \sec^3 (x^2 - 5x)$

   $g(x) = (\sec (x^2 - 5x))^3$

   $g'(x) = 3\sec^2 (x^2 - 5x) \dfrac{d}{dx} (\sec (x^2 - 5x))$

   $= 3\sec^2 (x^2 - 5x) \sec (x^2 - 5x) \tan (x^2 - 5x) . 2x$

   $= 6x \sec^3 (x^2 - 5x) \tan (x^2 - 5x)$

** Solution 7

   $f(x) = \cos^2 (3x)$

   $f'(x) = 2\cos (3x) - \sin (3x) 3$

   $= -6 \sin 3x \cos 3x$

** Solution 8

   $g(x) = \sqrt{\cos^2 (3x) + 1}$

   $g'(x) = \dfrac{1}{2} (\cos^2 (3x) + 1)^{-1/2} (-6\sin 3x \cos 3x)$ (From solution 7)

   $= \dfrac{-3 \sin 3x \cos 3x}{\sqrt{\cos^2 (3x) + 1}}$

** Solution 9

   $h(x) = x\sqrt[4]{2x + 3}$

   $h(x) = x(2x+3)^{1/4}$

   Using the product rule,

   $h'(x) = x \dfrac{d}{dx}(2x+3)^{1/4} + (2x+3)^{1/4}$

   $= \dfrac{x}{4}(2x+3)^{-3/4}2 + (2x+3)^{1/4}$

   $= \dfrac{x}{2\sqrt[4]{(2x+3)^3}} + \sqrt[4]{(2x+3)}$

** Solution 10

   $f(x) = x^2\sqrt[3]{3x-5}$

   $f(x) = x^2(3x-5)^{1/3}$

   Using the product rule,

   $f'(x) = x^2\dfrac{d}{dx}(3x-5)^{1/3} + 2x(3x-5)^{1/3}$

   $= x^2\dfrac{1}{3}(3x-5)^{-2/3} + 2x(3x-5)^{1/3}$

   $= \dfrac{x^2}{3\sqrt[3]{(3x-5)^2}} + 2x\sqrt[3]{3x-5}$

** Solution 11

   $g(x) = \sin (\cos (\tan (3x)))$

   $g'(x) = \cos (\cos (\tan (3x))) \dfrac{d}{dx} (\cos (\tan 3x))$

   $= \cos (\cos (\tan 3x)) * - \sin (\tan 3x) \dfrac{d}{dx} (\tan 3x)$

   $= \cos (\cos (\tan 3x)) * -\sin (\tan 3x) \sec^2 3x 3$

   $= -3 \sec^2 3x \sin(\tan 3x) \cos (\cos (\tan 3x))$

** Solution 12

   $h(x) = \sqrt{5 + 4\sqrt{3 + 2\sqrt{1+x}}}$

   $h(x) = (5 + 4\sqrt{3 + 2\sqrt{1+x}})^{1/2}$

   $h'(x) = \dfrac{1}{2}(5 + 4\sqrt{3 + 2\sqrt{1+x}})^{-1/2} \dfrac{d}{dx}(4\sqrt{3 + 2\sqrt{1+x}})$

   $= \dfrac{1}{2}(5+ 4\sqrt{3 + 2\sqrt{1+x}})^{-1/2} . 4(3+2\sqrt{1+2})^{-1/2} \dfrac{d}{dx} (2\sqrt{1+x})$

   $= 2(5+ 4\sqrt{3 + 2\sqrt{1+x}})^{-1/2} 4\sqrt{3 + 2\sqrt{1+x}} 2(1+x)^{-1/2}$

   $= \dfrac{4}{\sqrt{(5 + 4 \sqrt{3+2\sqrt{1+x}})}(\sqrt{3 + 2\sqrt{1+x}})\sqrt{1+x}}$

** Solution 13

   $f(x) = (\dfrac{2x+5}{2-5x})^7$

   $f(x) = (2x+5)^2(2-5x)^{-7}$

   Using the product rule,

   $f'(x) = (2x+5)^7\dfrac{d}{dx}(2-5x)^{-7} + (2-5x)^{-7} \dfrac{d}{dx} (2x+5)^7$

   $= (2x+5)^7.-7(2-5x)^{-8}(-5) + (2-5x)^{-7}.7(2x+5)^6.2$

   $= \dfrac{35(2x+5)^7}{(2-5x)^8} + \dfrac{14(2x+5)^6}{(2-5x)^7}$

** Solution 14

   $g(x) = \dfrac{\cos 5x}{\sin 3x}$

   $g(x) = \cos 5x \csc 3x$

   Using the product rule,

   $g'(x) = \cos 5x \dfrac{d}{dx} \csc (3x) + \csc (3x) \dfrac{d}{dx} (\cos 5x)$

   $= \cos 5x - \csc 3x \cot 3x . 3 + \csc 3x (-\sin 5x) . 5$

   $= -3\cos 5x \csc 3x - \cot 3x - 5\sin 5x \csc 3x$

** Solution 15

   $f(x) = \sqrt{\tan x}$

   $f'(x) = \dfrac{1}{2} (\tan x)^{-1/2} \sec^2 x$

   $= \dfrac{\sec^2 x}{2 \sqrt{\tan x}}$

** Solution 16

   $g(x) = \sqrt{\dfrac{x^2 - 1}{x^2 + 1}}$

   $g(x) = (x^2 - 1)^{1/2}(x^2 + 1)^{-1/2}$

   Using the product rule,

   $g'(x) = (x^2-1)^{1/2}\dfrac{d}{dx}(x^2+1)^{-1/2}+(x^2+1)^{-1/2}\dfrac{d}{dx}(x^2-1)^{1/2}$

   $= \dfrac{-1}{2}(x^2-1)^{1/2}(x^2+1)^{-3/2}(2x) + \dfrac{1}{2}(x^2+1)^{-1/2}(x^2-1)^{-1/2}(2x)$

   $= \dfrac{-x\sqrt{x^2-1}}{(x^2+1)^{3/2}} + \dfrac{x}{\sqrt{(x^2+1)(x^2-2)}}$

** Solution 17

   $g(x) = f(x^2-3x+1)$

   $f'(x)=3$

   $f''(1) = -1$

   Let $h=x^2-3x+1$

   $g(x) = f \circ h$

   Using chain rule,

   $g'(x) = f'(h(x))h'(x)$

   $h'(x) = 2x- 3$

   $g'(3) = f'(f(3))h'(3)$

   $h(3) = 3^2 - 3^2 + 1 = 1$

   $h'(3) = 3.2 - 3 = 3$

   $g'(3) = f'(1)h'(3)$

   $= 3.3 = 9$

   We know that,

   $g'(x) = f'(h(x))h'(x)$

   Using the product rule,

   $g''(x) = f'(h(x))h''(x) + h'(x)\dfrac{d}{dx}(f'(h(x)))$

   $= f'(h(x))h''(x) + h'(x)f''(h(x))h'(x)$

   $= f'(h(x))h''(x) + (h'(x))^2f''(h(x))$

   $g''(3) = f'(h(3))h''(3) + (h'(3))^2f''(h(3))$

   $h(3) = 1$

   $h'(3) = 3$

   $h''(x) = 2$

   $g''(3) = f'(1).2 + 3^2 f''(1)$

   $= 2f'(1)+9f''(1)$

   $=2.3 + 9(-1)$

   $= 6 - 9 = -3$

** Solution 18

   $y = 5x - 3$ is tangent to $y=f(x)$ at $(3,12)$

   $g(x) = \dfrac{f(x^2-1)}{x}$

   We need to find tangent for $y=g(x)$ at $(2,g(x))$

   $g(2) = \dfrac{f(4-1)}{3} = \dfrac{f(3)}{2}$

   We know that $f(3) = 12$

   $g(2) = \dfrac{12}{2} = 6$

   So we need to find tangent to $y=g(x)$ at $(2,6$)

   $g(x) = \dfrac{f(x^2-1)}{2}$

   $g'(x) = \dfrac{1}{2} \dfrac{d}{dx}f(x^2-1)$

   $= \dfrac{1}{2}f'(x^2-1)(2x)$

   $= xf'(x^2-1)$

   $g'(2) = 2f'(3) = 2.12 = 24$

   So we have the following data about the tangent:

   It's point: (2.6)

   It's slope = 24

   $y = mx + c$

   $6 = 24.2 + c$

   $c = 6 - 48 = -42$

   $y = 24x - 42$

** Solution 19

   $f(x) = (3x-2)^7$

   $f'(x) = 7(3x-2)^6(3)$

   $= 21(3x-2)^6$

   $f''(x) = 126(3x-2)^5$

   $= 378(3x-2)^5$

   $f'''(x) = 378.5(3x-2)^4$

   $= 1890(3x-2)^4$

** Solution 20

   $g(x) = \sec(3x + 1)$

   $g'(x) = \sec(3x + 1) \tan(3x+1).e$

   $g''(x) = 3\sec(3x+1)\dfrac{d}{dx}\tan(3x+1) + 3\tan(3x+1)\dfrac{d}{dx}\sec(3x+1)$

   $= 3\sec(3x+1)\sec^2(3x+1).3 + 3\tan(3x+1)\sec(3x+1)\tan(3x+1).3$

   $= 9\sec^3(3x + 1) + 9\tan^2(3x+1)\sec(3x + 1)$

   $g'''(x) = 27\sec^2(3x+1).3 + 9\tan^2(3x+1)\dfrac{d}{dx}\sec(3x+1) + 9\sec(3x+1)\dfrac{d}{dx}\tan^2(3x+1)$

   $= 27\sec^2(3x+1) + 9\tan^2(3x+1)\sec(3x+1)\tan(3x+1).3 + 9\sec(3x+1).2\tan(3x+1).3\sec^2(3x+1)$

   $= 27\sec^2(3x+1) + 27\tan^3(3x+1)\sec(3x+1) + 54\sec^3(3x+1)\tan(3x+1)$

** Solution 21

   $h(x) = \sin(2x)$

   $h'(x) = \cos(2x).2 = 2\cos (2x)$

   $h''(x) = -4\sin(2x)$

   $h'''(x) = -8\cos(2x)$

   $h''''(x) = 16\sin(2x)$

   So looking at the pattern, when we do differentiate 100th time,

   $h^{(100)}x = 2^{100}\sin(2x)$

** Solution 22

   $y = \sin(\pi t^2)$

   Velocity = $\dfrac{dy}{dt} = \cos (\pi t^2).2t\pi$

   $= 2t\pi\cos(\pi t^2)$

   Acceleration = $\dfrac{d^2y}{dt^2} = 2t\pi \dfrac{d}{dt} (\cos \pi t^2) + (\cos \pi t^2 \dfrac{d}{dt} (2t\pi))$

   $= -2\pi t\sin(\pi t^2)2\pi t + \pi t^2 (2\pi)$

   $= -4\pi^2t^2 \sin(\pi t^2) + 2\pi^2 t^2$

   $= 2\pi^2 t^2 - 4\pi^2t^2\sin(\pi t^2)$

   At $t=1$,

   Velocity = $2\pi(cos \pi) = -2\pi$

   Acceleration = $2\pi^2 - 4\pi^2\sin(\pi)$

   $= 2\pi^2 - 0 = 2\pi^2$

** Solution 23

   $\forall x \sin(2x) = 2\sin x \cos x$

   $2 \cos 2x = 2 \sin \dfrac{d}{dx}\cos x + 2 \cos x \dfrac{d}{dx} \sin x$

   $2\cos 2x = -2\sin x \sin x + 2\cos x \cos x$

   $2\cos 2x = -2\sin^2 x + 2\cos^2 x$

   $\cos 2x = \cos^2x - \sin^2 x$

** Solution 24

   $f(x) = x^{m/n}$

   $m$ and $n$ are positive integers.

   $m > n \geq 3$

   $n$ is odd.

   $m/n$ is reduced to lowest terms

   $y = x^{m/n}$

   $y^n = x^m$

   Differentiating above w.r.t x,

   $\dfrac{d}{dx}y^n = mx^{m-1}$

   $ny^{n-1}\dfrac{dy}{dx} = mx^{m-1}$

   $\dfrac{dy}{dx} = \dfrac{m(x^{m-1})}{ny^{n-1}}$

   $= \dfrac{mx^{m-1}}{n(x^{m/n})^{n-1}}$

   $= \dfrac{m}{n}x^{m-1-\dfrac{m(n-1)}{n}}$

   $= \dfrac{m}{n}x^{\dfrac{m}{n}-1}$

   Now since $m/n > 1$, we know that $m/n - 1 > 0$.

   So when $x=0$, the derivative is defined.

   $f'(0) = \dfrac{m}{n} 0^{m/n} = 0$

   
